\documentclass[12pt]{ociamthesis}  % default square logo 
%\documentclass[12pt,beltcrest]{ociamthesis} % use old belt crest logo
%\documentclass[12pt,shieldcrest]{ociamthesis} % use older shield crest logo

%load any additional packages
\usepackage{amssymb}
\usepackage{bbm}
%input macros (i.e. write your own macros file called mymacros.tex 
%and uncomment the next line)
%\include{mymacros}

\title{Modelling and analysis of social network data from rank preferences     %your thesis title,
	}   %note \\[1ex] is a line break in the title

\author{Pierre OSSELIN}             %your name
\college{St Peter's College}  %your college

%\renewcommand{\submittedtext}{change the default text here if needed}
\degree{MSc in Mathematical Sciences}     %the degree
\degreedate{Trinity 2018}         %the degree date

%end the preamble and start the document
\begin{document}
	
	
	\maketitle                  % create a title page from the preamble info
	
	
	
	%now include the files of latex for each of the chapters etc
	\section{Introduction}
	Hi How are you bruh?
	
	\section{Posterior}
	Let's define the posterior of the community representation.
	
	$l((w);D) = \sum_{i = 1}^{n} \sum_{k = 1}^{p} (\alpha - 1)ln(w_{i,k}) - \beta ln(w_{i,k}) + \sum_{i = 1}^{n} \sum_{j = 1}^{K} ln(\lambda_{i,\rho_{j}}) - ln(\sum_{j \neq i} \lambda_{i,j} - \sum_{l = 1}^{j-1} \lambda_{i,\rho_{l}})$
	
	To make the optimization easier, we can compute the gradient of the posterior according to the parameter $w_{r,s}$
	
	With $\frac{\partial \lambda_{i,j}}{\partial w_{r,s}} = 1_{i = r} w_{j,s} + 1_{j = r} w_{i,s}$
	
	We have :
	$\frac{\partial l((w);D)}{\partial w_{r,s}} = \frac{a-1}{w_{r,s}} - b 
	+ \sum_{j = 1}^{K} \frac{1}{\lambda_{r,\rho^{(r)}_{j}}} w_{\rho^{(r)}_{j},s} 
	+ \sum_{i = 1; i \neq r}^{n} \sum_{j = 1}^{K} \frac{1}{\lambda_{i,r}} w_{i,s} 1_{\rho^{(r)}_{j} = r}
	- \sum_{j = 1}^{K} \frac{1}{\sum_{j \neq r} \lambda_{r,j} - \sum_{l = 1}^{j - 1} \lambda_{r,\rho^{(r)}_{l}}} \sum_{j \neq r} w_{j,s}
	- \sum_{i = 1; i \neq r}^{n} \sum_{j = 1}^{K} \frac{1}{\sum_{j \neq i} \lambda_{i,j} - \sum_{l = 1}^{j - 1} \lambda_{i,\rho^{(i)}_{l}}} w_{i,s}$
	
	$ + \sum_{j = 1}^{K} \frac{1}{\sum_{j \neq r} \lambda_{r,j} - \sum_{l = 1}^{j - 1} \lambda_{r,\rho^{(r)}_{l}}} \sum_{l = 1}^{j-1} w_{\rho^{(r)}_{l},s}
	+ \sum_{i = 1; i \neq r}^{n} \sum_{j = 1}^{K} \frac{1}{\sum_{j \neq i} \lambda_{i,j} - \sum_{l = 1}^{j - 1} \lambda_{i,\rho^{(i)}_{l}}} \sum_{l = 1}^{j - 1} 1_{\rho^{(i)}_{l} = r} w_{i,s}$
	
	
	
	
	
\end{document}